feat(Keller): better lemma makes cleaner proofs

Experiments/Keller/SymmBreak/TwoCubes.lean
@@ -283,79 +283,75 @@ theorem c3_j₂ (tc : TwoCubes n s) : ∃ j₂ : Fin _, j₂.val ≥ 2 ∧ (tc.k
   rw [tc.c1]
   simp_all [Fin.ext_iff]
 
-def c3_2.auto (j₂ : Fin (n+5)) : KAuto (n+5) (s+2) :=
-  (KAuto.reorder (Equiv.Perm.setAll [(2, j₂)]))
+def c3_2.auto_equiv (j₂ : Fin (n+5)) := (Equiv.Perm.setAll [(2, j₂)])
 
-theorem c3_2.auto.app_0 {j₂ : Fin (n+5)} (j₂_ge : j₂.val ≥ 2) :
-      (Equiv.Perm.setAll [(2, j₂)]) 0 = 0 := by
+theorem c3_2.auto_equiv.app_0 {j₂ : Fin (n+5)} (j₂_ge : j₂.val ≥ 2) :
+      c3_2.auto_equiv j₂ 0 = 0 := by
   cases j₂; apply Equiv.Perm.setAll_eq_of_not_mem <;> simp_all [Fin.ext_iff]; omega
 
-theorem c3_2.auto.app_eq_0 {j₂ : Fin (n+5)} (j₂_ge : j₂ ≥ 2) {x} :
-      ((Equiv.Perm.setAll [(2, j₂)]) x : Nat) = 0 ↔ x = 0 := by
-  have := c3_2.auto.app_0 j₂_ge; simp [Fin.ext_iff] at this
-  rw [← this, ← Fin.ext_iff, Equiv.apply_eq_iff_eq]
+theorem c3_2.auto_equiv.symm_0 {j₂ : Fin (n+5)} (j₂_ge : j₂.val ≥ 2) :
+      (c3_2.auto_equiv j₂).symm 0 = 0 := by
+  rw [Equiv.symm_apply_eq, app_0 j₂_ge]
 
-theorem c3_2.auto.app_1 {j₂ : Fin (n+5)} (j₂_ge : j₂.val ≥ 2) :
-      (Equiv.Perm.setAll [(2, j₂)]) 1 = 1 := by
+theorem c3_2.auto_equiv.app_1 {j₂ : Fin (n+5)} (j₂_ge : j₂.val ≥ 2) :
+      c3_2.auto_equiv j₂ 1 = 1 := by
   cases j₂; apply Equiv.Perm.setAll_eq_of_not_mem <;> simp_all [Fin.ext_iff]; omega
 
-theorem c3_2.auto.app_eq_1 {j₂ : Fin (n+5)} (j₂_ge : j₂ ≥ 2) {x} :
-      ((Equiv.Perm.setAll [(2, j₂)]) x : Nat) = 1 ↔ x = 1 := by
-  have := c3_2.auto.app_1 j₂_ge; simp [Fin.ext_iff] at this
-  rw [← this, ← Fin.ext_iff, Equiv.apply_eq_iff_eq]
+theorem c3_2.auto_equiv.symm_1 {j₂ : Fin (n+5)} (j₂_ge : j₂.val ≥ 2) :
+      (c3_2.auto_equiv j₂).symm 1 = 1 := by
+  rw [Equiv.symm_apply_eq, app_1 j₂_ge]
+
+theorem c3_2.auto_equiv.above_2 {j₂ : Fin (n+5)} (j₂_ge : j₂.val ≥ 2) :
+      x ≥ 2 → (c3_2.auto_equiv j₂) x ≥ 2 := by
+  intro h
+  if x = 2 then
+    have : (auto_equiv j₂) x = j₂ :=
+      Equiv.Perm.setAll_eq_of_mem (by simp) (by simp) (by simp [*])
+    rw [this]; exact j₂_ge
+  else if x = j₂ then
+    have : (auto_equiv j₂) x = 2 := by
+      simp [auto_equiv, Equiv.Perm.setAll, Equiv.setAll, Equiv.setValue, *]
+    rw [this]
+  else
+    have : (auto_equiv j₂) x = x :=
+      Equiv.Perm.setAll_eq_of_not_mem (by simp [*]) (by simp [*])
+    rw [this]; exact h
 
 theorem c3_2.auto.maps_c3_2 (k : KClique (n+5) (s+2)) (j₂_ge : j₂.val ≥ 2)
-  : (KClique.map (c3_2.auto j₂) k |>.get 3)[2] = (k.get 3)[j₂] := by
-  -- give name to the new colors
-  generalize hcs : KClique.get _ _ = cs
-  rw [KClique.get_eq_iff_mem] at hcs
-  simp [KClique.map, c3_2.auto, KVertex.reorder] at hcs
-  rcases hcs with ⟨⟨pre_i,pre_cs⟩,v_mem,h,rfl⟩
+  : (KClique.map (KAuto.reorder <| c3_2.auto_equiv j₂) k |>.get 3)[2] = (k.get 3)[j₂] := by
+  rw [KClique.get_map_reorder]
   simp
-
-  -- in h we've uncovered a relationship between pre_i and 3
-  replace h : pre_i = 3#(n+3+2) := by
-    ext j hj
-    replace h := congrArg (·[(Equiv.Perm.setAll [(2, j₂)]).symm ⟨j,hj⟩]) h
-    simp at h; rw [h]; clear h
-    simp [bv_3_getElem, Fin.val_eq_iff_lt_and_eq, Equiv.symm_apply_eq,
-      c3_2.auto.app_0 j₂_ge, c3_2.auto.app_1 j₂_ge]
-    simp [Fin.ext_iff]
-
-  -- but now we know what pre_cs is too!
-  subst pre_i
-  rw [← KClique.get_eq_iff_mem] at v_mem
-  subst pre_cs
-
-  -- close the goal woohoo
-  congr
+  congr 2
+  ext i hi
+  simp only [bv_3_getElem, Fin.val_eq_iff_lt_and_eq, Fin.zero_eta, Equiv.symm_apply_eq,
+    c3_2.auto_equiv.app_0 j₂_ge, Fin.mk_one, c3_2.auto_equiv.app_1 j₂_ge]
+  simp [Fin.ext_iff]
 
 /-- We can always apply an automorphism to get a clique with c3[2] ≠ 0 -/
 theorem c3_2 (tc : TwoCubes (n+3) s) :
     ∃ tc' : TwoCubes (n+3) s, (tc'.kclique.get 3)[2] ≠ 0 := by
   have ⟨j₂, j₂_ge, spec⟩ := c3_j₂ tc
   refine ⟨{
-    kclique := tc.kclique.map (c3_2.auto j₂)
+    kclique := tc.kclique.map (KAuto.reorder <| c3_2.auto_equiv j₂)
     c0 := ?c0
     c1 := ?c1
   }, ?point⟩
   case c0 =>
-    rw [KClique.get_eq_iff_mem]
-    simp [KClique.map]
-    use ⟨0, tc.kclique.get 0⟩, tc.kclique.get_mem 0
-    ext j hj
-    · simp [c3_2.auto, KVertex.bv_reorder]
-    · simp [c3_2.auto, KVertex.colors_reorder, tc.c0_j]
+    simp [KClique.get_map_reorder]
+    suffices BitVec.ofFn _ = 0#(n+5) by
+      rw (occs := .pos [1]) [this]
+      ext; simp
+    ext1; simp
   case c1 =>
-    rw [KClique.get_eq_iff_mem]
-    simp [KClique.map]
-    use ⟨1, tc.kclique.get 1⟩, tc.kclique.get_mem 1
-    ext j hj
-    · have := c3_2.auto.app_eq_0 j₂_ge (x := ⟨j,hj⟩)
-      simp [Fin.ext_iff] at this
-      simp [c3_2.auto, KVertex.bv_reorder, this]
-    · have := c3_2.auto.app_eq_1 j₂_ge (x := ⟨j,hj⟩)
-      simp [c3_2.auto, KVertex.colors_reorder, tc.c1_j, this, Fin.ext_iff]
+    rw [KClique.get_map_reorder]
+    suffices BitVec.ofFn _ = 1#(n+5) by
+      rw [this]
+      ext; simp
+      simp [Fin.val_eq_iff_lt_and_eq, Equiv.apply_eq_iff_eq_symm_apply, c3_2.auto_equiv.symm_1 j₂_ge]
+      simp [Fin.ext_iff]
+    ext1 j hj
+    simp [Fin.val_eq_iff_lt_and_eq, Equiv.symm_apply_eq, c3_2.auto_equiv.app_0 j₂_ge]
+    simp [Fin.ext_iff]
   case point =>
     -- the new c3[2] should be the old c3[j₂]
     convert spec; clear spec
@@ -417,6 +413,8 @@ theorem ofTwoCubes (tc : TwoCubes (n+3) s) : Nonempty (ThreeCubes n s) :=
           Equiv.Perm.setAll [(1, (tc4.kclique.get 3)[2])]
         else Equiv.refl _
       )
+    c0 := by sorry
+    c1 := by sorry
     c3 := by intro i h; simp; sorry
   }⟩
 
